bedrock2/src/Examples/ipow.v
@@ -1,7 +1,3 @@
-Ltac head expr :=
-  match expr with  | ?f _ => head f
-  | _ => expr
-  end.
 Ltac rdelta x :=
   match constr:(Set) with
   | _ => let x := eval unfold x in x in x
@@ -37,9 +33,30 @@ Definition invert_Some {A} (x : option A) : match x with
      | None => tt
      end.
 
+Set Printing Depth 999999.
+Local Notation "'need!' y 's.t.' Px 'let' x ':=' v 'using' pfPx 'in' pfP" :=
+  (let x := v in ex_intro (fun y => Px /\ _) x (conj pfPx pfP))
+  (right associativity, at level 200, pfPx at next level,
+    format "'need!'  y  's.t.'  Px  '/' 'let'  x  ':='  v  'using'  pfPx  'in'  '/' pfP").
+Local Notation "'need!' x 's.t.' Px 'let' x ':=' v 'using' pfPx 'in' pfP" :=
+  (let x := v in ex_intro (fun x => Px /\ _) x (conj pfPx pfP))
+  (only printing, right associativity, at level 200, pfPx at next level,
+    format "'need!'  x  's.t.'  Px  '/' 'let'  x  ':='  v  'using'  pfPx  'in'  '/' pfP").
+Local Notation "'need!' y 's.t.' Px 'let' x ':=' v 'using' pfPx 'in' pfP" :=
+  (let x := v in ex_intro (fun y => Px /\ _) x (conj pfPx pfP))
+  (right associativity, at level 200, pfPx at next level,
+   format "'need!'  y  's.t.'  Px  '/' 'let'  x  ':='  v  'using'  pfPx  'in'  '/' pfP")
+  : type_scope.
+Local Notation "'need!' x 's.t.' Px 'let' x ':=' v 'using' pfPx 'in' pfP" :=
+  (let x := v in ex_intro (fun x => Px /\ _) x (conj pfPx pfP))
+  (only printing, right associativity, at level 200, pfPx at next level,
+   format "'need!'  x  's.t.'  Px  '/' 'let'  x  ':='  v  'using'  pfPx  'in'  '/' pfP")
+  : type_scope.
+
 
 Require Import bedrock2.Macros bedrock2.Syntax.
 Require Import bedrock2.BasicC64Syntax bedrock2.BasicALU bedrock2.NotationsInConstr.
+
 
 Import BinInt String List.ListNotations.
 Local Open Scope string_scope. Local Open Scope Z_scope. Local Open Scope list_scope.
@@ -63,6 +80,14 @@ Require Import bedrock2.Map.Separation bedrock2.Map.SeparationLogic.
 Require bedrock2.WeakestPrecondition bedrock2.WeakestPreconditionProperties.
 Require bedrock2.TailRecursion.
 
+Lemma shiftr_decreases
+      (x1 : Word.word 64)
+      (n : Word.wzero 64 <> x1)
+  : (Word.wordToNat (Word.wrshift' x1 1) < Word.wordToNat x1)%nat.
+  cbv [Word.wrshift'].
+Admitted.
+Lemma word_test_true w : word_test w = true -> w <> Word.wzero 64. Admitted.
+
 Section WithT.
   Context {T : Type}.
   Fixpoint bindcmd (c : cmd) (k : cmd -> T) {struct c} : T :=
@@ -70,34 +95,15 @@ Section WithT.
     | cmd.cond e c1 c2 => bindcmd c1 (fun c1 => bindcmd c2 (fun c2 => let c := cmd.cond e c1 c2 in k c))
     | cmd.seq c1 c2 => bindcmd c1 (fun c1 => bindcmd c2 (fun c2 => let c := cmd.seq c1 c2 in k c))
     | cmd.while e c => bindcmd c (fun c => let c := cmd.while e c in k c)
-    | c => let c := c in k c
+    | c => k c
     end.
 End WithT.
 
 Definition spec_of_ipow := fun functions =>
   forall x e t m,
     WeakestPrecondition.call (fun _ => True) (fun _ => False) (fun _ _ => False) functions
-      (fst ipow) t m [x; e]
+      "ipow" t m [x; e]
       (fun t' m' rets => t=t'/\ m=m' /\ exists v, rets = [v]).
-
-(* FIXME: this may reduce in the values as well *)
-Ltac reduce_locals_map :=
-cbv [
-    locals parameters
-    map.put map.get map.empty map.putmany invert_Some
-    SortedListString.map
-    SortedList.parameters.key SortedList.parameters.value
-    SortedList.parameters.key_eqb SortedList.parameters.key_ltb
-    SortedList.map SortedList.sorted SortedList.put
-    SortedList.value SortedList.ok SortedList.minimize_eq_proof
-    String.eqb String.ltb String.prefix
-    Ascii.eqb Ascii.ltb Ascii.ascii_dec Ascii.ascii_rec Ascii.ascii_rect
-    Ascii.N_of_ascii Ascii.N_of_digits
-    BinNatDef.N.ltb BinNatDef.N.eqb BinNatDef.N.compare BinNat.N.add BinNat.N.mul
-    Pos.mul Pos.add Pos.eqb Pos.ltb Pos.compare Pos.compare_cont
-    Bool.bool_dec bool_rec bool_rect sumbool_rec sumbool_rect
-    andb orb
-  ].
 
 Ltac bind_body_of_function f_ :=
   let f := eval cbv in f_ in
@@ -113,7 +119,6 @@ Ltac bind_body_of_function f_ :=
   cbv beta iota delta [bindcmd]; intros.
 
 Import WeakestPrecondition.
-(* FIXME: do not perform beta+iota reduction in non-recursive arguments *)
 Ltac unfold1_wp_cmd e :=
   lazymatch e with
     @cmd ?params ?R ?G ?PR ?CA ?c ?t ?m ?l ?post =>
@@ -147,36 +152,107 @@ Ltac unfold1_list_map_goal :=
   let G := unfold1_list_map G in
   change G.
 
-Ltac straightline :=
+Ltac is_nat_literal x :=
+  lazymatch x with
+  | O => idtac
+  | S ?x => is_nat_literal x
+  end.
+
+Ltac refine_ex :=
+  hnf;
+  lazymatch goal with
+  | |- exists x, ?P =>
+    let x := fresh x in
+    refine (let x := _ in ex_intro (fun x => P) x _)
+  end.
+
+Ltac straightline_cleanup :=
   match goal with
+  | x := _ |- _ =>
+         assert_succeeds (clear x);
+           match type of x  with
+           | unit => clear x
+           | bool => clear x
+           | list _ => clear x
+           | nat => clear x
+           | word => clear x
+           | map.rep => clear x
+           | cmd.cmd => clear x
+           | expr.expr => clear x
+           end
+
+  | |- @HList.tuple.foralls ?A ?n (fun x => ?P) =>
+    let n := eval hnf in n in
+    lazymatch n with
+    | O => change (subst! tt for x in P)
+    | S ?n' =>
+      let a := fresh x in
+      let y := fresh x in
+      change (forall a:A, @HList.tuple.foralls A n' (fun y => subst! (PrimitivePair.pair.mk a y) for x in P))
+    end
+  | |- @HList.hlist.foralls ?l (fun x => ?P) =>
+    let l := eval hnf in l in
+    lazymatch l with
+    | nil => change (subst! tt for x in P)
+    | cons ?A ?ts' =>
+      let a := fresh x in
+      let y := fresh x in
+      change (forall a:A, @HList.hlist.foralls ?ts' (fun y => subst! (PrimitivePair.pair.mk a y) for x in P))
+    end
+  | |- @HList.tuple.foralls ?A ?n ?P =>
+    let n' := eval hnf in n in
+    is_nat_literal n'; change (@HList.tuple.foralls A n' P)
+
+  (* bad implementations of reductions that reduce let binders, user sparingly *)
+  | H: PrimitivePair.pair._1 (HList.tuple.apply _ _) |- _ =>
+    cbn [List.repeat Datatypes.length HList.tuple.apply PrimitivePair.pair._1 PrimitivePair.pair._2] in H
+  | |- PrimitivePair.pair._1 (HList.tuple.apply _ _) =>
+    cbn [List.repeat Datatypes.length HList.tuple.apply PrimitivePair.pair._1 PrimitivePair.pair._2]
+  | H: HList.tuple.apply (PrimitivePair.pair._2 _ _ _) _ |- _ =>
+    cbn [List.repeat Datatypes.length HList.tuple.apply PrimitivePair.pair._1 PrimitivePair.pair._2] in H
+  | |- HList.tuple.apply (PrimitivePair.pair._2 _ _ _) _ =>
+    cbn [List.repeat Datatypes.length HList.tuple.apply PrimitivePair.pair._1 PrimitivePair.pair._2]
+  | |- context [@HList.hlist.existss] => progress (cbv beta iota delta [HList.hlist.existss])
+
   | |- forall _, _ => intros
   | |- let _ := _ in _ => intros
-  | x := ?y |- ?G => is_var y; subst x
-  | _ => progress cbv iota beta in *
   | H: exists _, _ |- _ => destruct H
   | H: _ /\ _ |- _ => destruct H
+  | x := ?y |- ?G => is_var y; subst x
+  | H : ?x = ?y |- _ => constr_eq x y; clear H
   | H: ?x = ?v |- _ =>
-    assert_succeeds (subst x);
+    is_var x;
+    lazymatch v with context[x] => fail | _ => idtac end;
     let x' := fresh "x" in
     rename x into x';
     simple refine (let x := v in _);
     change (x' = x) in H;
     symmetry in H;
     destruct H
+  end.
+
+Ltac straightline :=
+  match goal with
+  | _ => straightline_cleanup
   | |- @cmd _ _ _ _ _ ?c _ _ _ ?post =>
     let c := eval hnf in c in
-    assert_fails (idtac; lazymatch c with cmd.while _ _ => idtac end);
-    unfold1_wp_cmd_goal; cbv beta match delta [cmd_body]
+    lazymatch c with
+    | cmd.while _ _ => fail
+    | cmd.cond _ _ _ => fail
+    | _ => unfold1_wp_cmd_goal; cbv beta match delta [cmd_body]
+    end
   | |- @list_map _ _ (@get _ _) _ _ => unfold1_list_map_goal; cbv beta match delta [list_map_body]
   | |- @list_map _ _ (@expr _ _ _) _ _ => unfold1_list_map_goal; cbv beta match delta [list_map_body]
+  | |- @list_map _ _ _ nil _ => cbv beta match fix delta [list_map list_map_body]
   | |- @expr _ _ _ _ _ => unfold1_wp_expr_goal; cbv beta match delta [expr_body]
   | |- @dexpr _ _ _ _ _ => cbv beta delta [dexpr] (* TODO: eabstract (repeat straightline) *)
   | |- @literal _ _ _ => cbv beta delta [literal]
   | |- @get _ _ _ _ => cbv beta delta [get]
+  | |- TailRecursion.enforce _ _ _ => exact (conj eq_refl eq_refl)
   | |- word_of_Z ?z = Some ?v =>
     let v := rdelta v in is_evar v; (change (word_of_Z z = Some v)); exact eq_refl
   | |- @eq (@map.rep _ _ (@locals _)) _ _ =>
-    eapply SortedList.eq_value; reduce_locals_map; exact eq_refl
+    eapply SortedList.eq_value; exact eq_refl
   | |- @map.get _ _ (@locals _) _ _ = Some ?v =>
     let v' := rdelta v in is_evar v'; (change v with v'); exact eq_refl
   | |- ?x = ?y =>
@@ -185,79 +261,76 @@ Ltac straightline :=
     let x := rdelta x in is_evar x; change (x=y); exact eq_refl
   | |- ?x = ?y =>
     let x := rdelta x in let y := rdelta y in constr_eq x y; exact eq_refl
-  | |- exists x, ?P =>
-    let x := fresh x in refine (let x := _ in ex_intro (fun x => P) x _)
-  | |- ?P /\ ?Q => refine (@conj P Q _ _)
+  | |- exists x, ?P /\ ?Q =>
+    let x := fresh x in refine (let x := _ in ex_intro (fun x => P /\ Q) x _);
+                        split; [solve [repeat straightline]|]
+  | |- exists x, Markers.split (?P /\ ?Q) =>
+    let x := fresh x in refine (let x := _ in ex_intro (fun x => P /\ Q) x _);
+                        split; [solve [repeat straightline]|]
+  | |- Markers.unique (exists x, Markers.split (?P /\ ?Q)) =>
+    let x := fresh x in refine (let x := _ in ex_intro (fun x => P /\ Q) x _);
+                        split; [solve [repeat straightline]|]
+  | |- Markers.unique (Markers.left _) =>
+    unshelve (idtac; repeat match goal with
+                     | |- Markers.split (?P /\ Markers.right ?Q) =>
+                       split; [eabstract (repeat straightline) | change Q]
+                     | _ => refine_ex
+                     end); []
+  | |- Markers.split ?G => change (G); split
   | |- True => exact I
   | |- False \/ _ => right
   | |- _ \/ False => left
   end.
 
-Notation "'letlocals' x .. y := vs 'in' p" :=
-  (fun l => ex (fun x => .. (ex (fun y =>
-    l = invert_Some (map.putmany vs (cons x .. (cons y nil) .. ) map.empty)
-    /\ p)) ..))
-  (at level 200, x binder, right associativity)
-  : type_scope.
+Ltac show_program :=
+  lazymatch goal with
+  | |- @cmd ?A ?B ?C ?D ?E ?c ?F ?G ?H ?I =>
+    let c' := eval cbv in c in
+    change (@cmd A B C D E (fst (c, c')) F G H I)
+  end.
 
-Set Printing Depth 999999.
-Local Notation "'need!' y 's.t.' Px 'let' x ':=' v 'using' pfPx 'in' pfP" :=
-  (let x := v in ex_intro (fun y => Px /\ _) x (conj pfPx pfP))
-  (right associativity, at level 200, pfPx at next level,
-    format "'need!'  y  's.t.'  Px  '/' 'let'  x  ':='  v  'using'  pfPx  'in'  '/' pfP").
-Local Notation "'need!' x 's.t.' Px 'let' x ':=' v 'using' pfPx 'in' pfP" :=
-  (let x := v in ex_intro (fun x => Px /\ _) x (conj pfPx pfP))
-  (only printing, right associativity, at level 200, pfPx at next level,
-    format "'need!'  x  's.t.'  Px  '/' 'let'  x  ':='  v  'using'  pfPx  'in'  '/' pfP").
-Local Notation "'need!' y 's.t.' Px 'let' x ':=' v 'using' pfPx 'in' pfP" :=
-  (let x := v in ex_intro (fun y => Px /\ _) x (conj pfPx pfP))
-  (right associativity, at level 200, pfPx at next level,
-   format "'need!'  y  's.t.'  Px  '/' 'let'  x  ':='  v  'using'  pfPx  'in'  '/' pfP")
-  : type_scope.
-Local Notation "'need!' x 's.t.' Px 'let' x ':=' v 'using' pfPx 'in' pfP" :=
-  (let x := v in ex_intro (fun x => Px /\ _) x (conj pfPx pfP))
-  (only printing, right associativity, at level 200, pfPx at next level,
-   format "'need!'  x  's.t.'  Px  '/' 'let'  x  ':='  v  'using'  pfPx  'in'  '/' pfP")
-  : type_scope.
-
-Lemma shiftr_decreases
-      (x1 : Word.word 64)
-      (n : Word.wzero 64 <> x1)
-  : (Word.wordToNat (Word.wrshift' x1 1) < Word.wordToNat x1)%nat.
-  SearchAbout Word.wrshift'.
-  cbv [Word.wrshift'].
-Admitted.
-Lemma word_test_true w : word_test w = true -> w <> Word.wzero 64. Admitted.
+Import TailRecursion PrimitivePair HList hlist tuple pair.
 
 Lemma ipow_ok : forall functions, spec_of_ipow (ipow::functions).
 Proof.
   bind_body_of_function ipow; cbv [spec_of_ipow].
-  intros x0 e0 t0 m0; hnf.
-  repeat straightline. { exact eq_refl. }
+  intros.
+  hnf. (* incoming call dispatch *)
+  eexists. split. exact eq_refl. (* argument initialization *)
 
-  refine (let P_ := fun v t m =>
-    letlocals x e ret := ["x"; "e"; "ret"] in v = Word.wordToNat e /\ t = t0 /\ m = m0 in _).
-  refine (let Q_ := fun v t m =>
-    letlocals x e ret := ["x";"e";"ret"] in t = t0 /\ m = m0 in _).
-  eapply TailRecursion.tailrec with (lt:=lt) (P:=P_) (Q:=Q_).
+  repeat straightline; show_program.
 
+  refine (TailRecursion.tailrec nil [("e":Syntax.varname);"ret";"x"]
+    (fun v t m e ret x => pair.mk (v = Word.wordToNat e)
+    (fun t' m' e' ret' x' => t' = t /\ m' = m))
+    lt _ _ tt _ _ _).
+
+  { split. exact eq_refl. eapply SortedList.eq_value. exact eq_refl. } (* init locals *)
   { exact Wf_nat.lt_wf. }
-  { subst P_. repeat straightline. }
-  { intros; cbv [P_ Q_] in * |-.
-    repeat straightline; subst P_; subst Q_; repeat straightline.
-    (* measure decreases *)
-    { cbn [interp_binop parameters] in *.
-      eapply word_test_true in H.
-      eapply shiftr_decreases. congruence. }
-    { cbn [interp_binop parameters] in *.
-      eapply word_test_true in H.
-      eapply shiftr_decreases. congruence. }
-  }
+  { repeat straightline. } (* init precondition *)
+  { (* loop test *)
+    repeat straightline; try show_program.
+    { (* loop body *)
+      refine_ex; split; [eabstract (repeat straightline)|]. (* if condition *)
+      split. (* if cases, path-blasting *)
+      { repeat straightline.
+        { (* measure decreases *)
+          cbn [interp_binop parameters] in *.
+          repeat match goal with H: word_test _ = true |- _ => eapply word_test_true in H end.
+          eapply shiftr_decreases. congruence. }
+        { split; exact eq_refl. } }
+      { repeat straightline.
+        { (* measure decreases *)
+          cbn [interp_binop parameters] in *.
+          repeat match goal with H: word_test _ = true |- _ => eapply word_test_true in H end.
+          eapply shiftr_decreases. congruence. }
+        { split; exact eq_refl. } } }
+    { (* end of loop *)
+      split; exact eq_refl. } }
 
-  subst Q_. repeat straightline.
-  unfold1_list_map_goal; cbv beta iota delta [list_map_body]; repeat straightline.
-  exact eq_refl.
+  repeat straightline.
 
-  Unshelve.
-  eapply WeakestPreconditionProperties.Proper_call; cbv; intuition idtac.
+  (* function postcondition *)
+  repeat eapply conj; try exact eq_refl.
+  eexists; exact eq_refl.
 Defined.
