bedrock2/src/Markers.v
@@ -1,0 +1,15 @@
+Local Set Universe Polymorphism.
+Section WithT.
+  Context {T : Type}.
+  Implicit Types x : T.
+  Definition intro x := x.
+  Definition split x := x.
+  Definition esplit x := x.
+  Definition econstructor x := x.
+  Definition exact_eq_refl x := x.
+  Definition exfalso x := x.
+
+  Definition unique x := x.
+  Definition left x := x.
+  Definition right x := x.
+End WithT.
