bedrock2/src/PrimitivePair.v
@@ -1,0 +1,21 @@
+Module pair.
+  Local Set Universe Polymorphism.
+  Local Set Primitive Projections.
+  Record pair {A B} := mk { _1 : A; _2 : B _1 }.
+  Arguments pair : clear implicits.
+  Arguments mk {A B} _ _.
+
+  (* TODO: make * right-associative like /\ *)
+  Notation "A * B" := (pair A%type (fun _ => B%type)) : type_scope.
+
+  Notation "{ x  &  P }" := (pair _ (fun x => P)) : type_scope.
+  Notation "{ ' pat  &  P }" := (pair _ (fun pat => P)) : type_scope.
+
+  Notation "{ x : A  &  P }" := (pair A (fun x => P)) : type_scope.
+  Notation "{ ' pat : A  &  P }" := (pair A (fun pat => P)) : type_scope. 
+
+  Notation "( x , y , .. , z )" := (mk .. (mk x y) .. z) : core_scope.
+
+  Notation "x '.(1)'" := (_1 x) (at level 1, left associativity) : core_scope.
+  Notation "x '.(2)'" := (_2 x) (at level 1, left associativity) : core_scope.
+End pair. Notation pair := pair.pair.
